proof/proof_addition.v
@@ -59,3 +59,86 @@ Proof.
     + apply bits_word_to_nat_of_nat2.
     + reflexivity.
 Defined.
+
+Require koika.riscv.
+Require sail.riscv.
+Require sail.riscv_types.
+
+Locate alu32.
+
+Definition koika_eval
+  { reg_t : Type }
+ `{ FiniteType reg_t }
+  { sig : tsig var_t }
+  { tau }
+  { R : reg_t -> type }
+  ( env: env_t ContextEnv R )
+  ( func : action R empty_Sigma sig tau )
+  ( inputs : input )
+  (* : option ((ContextEnv) * tau) *) :=
+    match (interp_action env empty_sigma inputs log_empty log_empty func) with
+    | Some (log,out,_) =>
+      let ctxt := commit_update env log in
+      Some (ctxt,out)
+    | None => None
+    end.
+
+(* Definition convert_tuple {A B} : (A * B) ->  *)
+
+Notation "(( a , .. , b ))" :=
+  (CtxCons (_,_) a .. (CtxCons (_,_) b CtxEmpty) ..)
+  (at level 0, 
+  a constr at level 80,
+  b constr at level 80).
+
+Definition sail_eval {A B C D E} (func : A -> B -> C -> D -> E) (inp : A * B * C * D) :=
+  let '(a,b,c,d) := inp in
+  func a b c d.
+
+Notation "a '=nat' b" := (@eq nat (a : bits _) (b : mword _) ) (at level 69).
+
+Theorem addition_refinement_general:
+  forall a b r,
+
+  (* let koika_in :=  #{
+    ("funct3", bits_t 3) => koika.riscv.funct3_ADD;
+    ("funct7", bits_t 7) => koika.riscv.funct7_ADD;
+    ("b", bits_t 32) => (Bits.of_nat 32 b);
+    ("a", bits_t 32) => (Bits.of_nat 32 a)
+  }# in *)
+
+  let koika_in := ((
+    koika.riscv.funct3_ADD,
+    koika.riscv.funct7_ADD,
+    Bits.of_nat 32 a,
+    Bits.of_nat 32 b
+  )) : context _ (int_argspec koika.riscv.alu32') in
+
+  let sail_in := (
+    sail.riscv_types.funct3_ADD,
+    sail.riscv_types.funct7_ADD,
+    Word.natToWord 32 a,
+    Word.natToWord 32 b
+  ) in
+
+  assert Some (r', koika_out) := (koika_eval r koika.riscv.alu32 koika_in) in
+  let sail_out := sail_eval sail.riscv.alu32 sail_in in
+
+  (forall reg, r.[reg] = r'.[reg]) /\
+  koika_out =nat sail_out.
+Proof.
+  intros.
+  unfold sail_in, sail_eval.
+  simpl (sail.riscv.alu32 _ _ _ _).
+  unfold koika_eval.
+  unfold koika.riscv.alu32.
+  vm_compute (extract_success _ _).
+  unfold interp_action.
+  simpl.
+  split.
+  - intro reg.
+    destruct reg.
+  - apply bits_word_add.
+    + apply bits_word_to_nat_of_nat2.
+    + apply bits_word_to_nat_of_nat2.
+Defined.
