koika/riscv.v
@@ -1,0 +1,61 @@
+Require Import Koika.Frontend.
+
+Inductive reg_t :=.
+
+Definition funct3_ADD  := Ob~0~0~0.
+Definition funct7_ADD  := Ob~0~0~0~0~0~0~0.
+
+Definition funct3_SUB  := Ob~0~0~0.
+Definition funct7_SUB  := Ob~0~1~0~0~0~0~0.
+
+Definition funct3_SLL  := Ob~0~0~1.
+Definition funct7_SLL  := Ob~0~0~0~0~0~0~0.
+
+Definition funct3_SLT  := Ob~0~1~0.
+Definition funct7_SLT  := Ob~0~0~0~0~0~0~0.
+
+Definition funct3_SLTU := Ob~0~1~1.
+Definition funct7_SLTU := Ob~0~0~0~0~0~0~0.
+
+Definition funct3_XOR  := Ob~1~0~0.
+Definition funct7_XOR  := Ob~0~0~0~0~0~0~0.
+
+Definition funct3_SRL  := Ob~1~0~1.
+Definition funct7_SRL  := Ob~0~0~0~0~0~0~0.
+
+Definition funct3_SRA  := Ob~1~0~1.
+Definition funct7_SRA  := Ob~0~1~0~0~0~0~0.
+
+Definition funct3_OR   := Ob~1~1~0.
+Definition funct7_OR   := Ob~0~0~0~0~0~0~0.
+
+Definition funct3_AND  := Ob~1~1~1.
+Definition funct7_AND  := Ob~0~0~0~0~0~0~0.
+
+
+Definition R (r : reg_t) : type :=
+  match r with
+  end.
+
+Definition alu32' : UInternalFunction reg_t empty_ext_fn_t := {{
+fun alu32 (funct3 : bits_t 3) (funct7 : bits_t 7)
+  (a : bits_t 32) (b : bits_t 32) : bits_t 32 =>
+    let shamt := b[Ob~0~0~0~0~0 :+ 5] in
+    let inst_30 := funct7[|3`d5|] in
+    match funct3 with
+    | #funct3_ADD  => if (inst_30 == Ob~1) then
+                      a - b
+                    else
+                      a + b
+    | #funct3_SLL  => a << shamt
+    | #funct3_SLT  => zeroExtend(a <s b, 32)
+    | #funct3_SLTU => zeroExtend(a < b, 32)
+    | #funct3_XOR  => a ^ b
+    | #funct3_SRL  => if (inst_30 == Ob~1) then a >>> shamt else a >> shamt
+    | #funct3_OR   => a || b
+    | #funct3_AND  => a && b
+    return default: #(Bits.of_nat 32 0)
+    end
+}}.
+
+Definition alu32 := tc_function R empty_Sigma alu32'.
