proof/proof_some_func.v
@@ -1,0 +1,88 @@
+Require sail.sail.
+Require sail.sail_types.
+Require koika.koika.
+Require Import Prelude.
+Require Import Koika.Frontend.
+Require Import Koika.Testing.
+Require Import Sail.Base.
+(* Require Import Sail.Values. *)
+Require Import Sail.State_lifting.
+Require Import Sail.State_monad.
+Require Import Nat.
+Require Import proof.proof_common.
+
+Require Import List.
+Import List.ListNotations.
+
+Definition koika_env_idk  :=
+  (fun n1 n2 =>
+  #{
+      koika.SOME_REG    => Bits.of_nat 32 n2;
+      koika.ANOTHER_REG => Bits.of_nat 16 n1
+  }#
+  ) : forall (n1 n2 : nat),  ContextEnv.(env_t) (fun (x : koika.reg_t) => koika.R x).
+
+Definition input { sig : list (string * type) } := context ( fun (x : (string * type)) => (snd x) ) sig.
+
+Check (#{ ("value", bits_t 32) => (Bits.of_nat 32 89) }# : input).
+
+Check (fun n_ar n_sr => (#{
+  koika.SOME_REG    => Bits.of_nat 32 n_sr;
+  koika.ANOTHER_REG => Bits.of_nat 16 n_ar
+}# : context koika.R _ ) : ContextEnv.(env_t) koika.R ).
+
+Theorem idk:
+  forall (n_in : nat) (koika_r : ContextEnv.(env_t) koika.R),
+
+  let koika_in : input := #{ ("value", bits_t 32) => (Bits.of_nat 32 n_in) }# in
+
+  (* let koika_r :=
+  (#{
+    koika.SOME_REG    => Bits.of_nat 32 50;
+    koika.ANOTHER_REG => Bits.of_nat 16 50
+  }# : context koika.R _ ) : ContextEnv.(env_t) koika.R in *)
+
+  True.
+Proof. intros. exact I. Defined.
+
+Notation "s 's=k' k" := (sail_koika_reg_eq s k) (no associativity,at level 69).
+
+Theorem some_func_equality:
+  forall (n : nat)
+    (koika_r : ContextEnv.(env_t) koika.R)
+    (sail_r : sail_types.regstate),
+
+  let koika_in := #{ ("value", bits_t 32) => (Bits.of_nat 32 n) }# in
+  let sail_in  := Word.natToWord 32 n in
+
+  sail_r s=k koika_r ->
+
+  (* koika *)
+  assert Some (koika_r', koika_out) :=
+    koika_eval koika_r koika.some_func_tc koika_in in
+  (* sail *)
+  assert [(Value sail_out,{|ss_regstate := sail_r'|},_)] :=
+    sail_eval sail_r sail.some_func sail_in in
+
+  (* actual condition *)
+  Bits.to_nat koika_out = Word.wordToNat sail_out  /\
+  sail_r' s=k koika_r'.
+Proof.
+  intros.
+  unfold koika_eval, sail_eval.
+
+  (* cbn in koika_r. *)
+  simpl (interp_action _ _ _ _ _ _).
+  cbv match.
+  cbn.
+  split.
+  - apply bits_word_add.
+    + unfold sail_in.
+      apply bits_word_to_nat_of_nat.
+      reflexivity.
+    + unfold sail_koika_reg_eq in H.
+      exact (H koika.SOME_REG).
+  - unfold sail_koika_reg_eq.
+    intro reg.
+    exact (H reg).
+Defined.
